Auto/Embedding/LCtx.lean
@@ -723,7 +723,7 @@ section push
     dsimp [pushLCtxsAtDep]; apply restoreAtDep_succ_succ_Fn
 
   theorem List.ofFun_get?_eq_none (f : Nat → α) (n m : Nat) (h : n ≤ m) :
-    (List.ofFun f n).get? m = .none := by
+    (List.ofFun f n)[m]? = .none := by
     induction m generalizing f n
     case zero =>
       cases n
@@ -859,7 +859,7 @@ section pushs_pops
     rw [List.ofFun_length]
     match h : Nat.blt n lvl with
     | true =>
-      rw [List.ofFun_get?_eq_some]; rfl
+      rw [ List.ofFun_getElem?_eq_some]; rfl
       dsimp [Nat.blt] at h;
       exact Nat.le_of_ble_eq_true h
     | false =>
